    \begin{equation}
    \int \frac{1}{a^2+x^2}dx = \frac{1}{a}\tan^{-1}\frac{x}{a}
    \end{equation}
    
    \begin{equation}
    \int \frac{x}{a^2+x^2}dx = \frac{1}{2}\ln|a^2+x^2|
    \end{equation}
    
    \begin{equation}
    \int \frac{1}{ax^2+bx+c}dx = \frac{2}{\sqrt{4ac-b^2}}\tan^{-1}\frac{2ax+b}{\sqrt{4ac-b^2}}
    \end{equation}
    
    \begin{equation}
    \int \frac{1}{(x+a)(x+b)}dx = \frac{1}{b-a}\ln\frac{a+x}{b+x}, \text{ } a\ne b
    \end{equation}
    
    \begin{equation}
    \int\sqrt{x^2 \pm a^2}\ dx = \frac{1}{2}x\sqrt{x^2\pm a^2} 
    \pm\frac{1}{2}a^2 \ln \left | x + \sqrt{x^2\pm a^2} \right | 
    \end{equation}
    
    \begin{equation}
    \int  \sqrt{a^2 - x^2}\ dx = \frac{1}{2} x \sqrt{a^2-x^2} 
    +\frac{1}{2}a^2\tan^{-1}\frac{x}{\sqrt{a^2-x^2}}
    \end{equation}
    
    \begin{equation}
    \int  x \sqrt{x^2 \pm a^2}\ dx= \frac{1}{3}\left ( x^2 \pm a^2 \right)^{3/2} 
    \end{equation}
    
    \begin{equation}
    \int \frac{1}{\sqrt{x^2 \pm a^2}}\ dx = \ln \left | x + \sqrt{x^2 \pm a^2} \right | 
    \end{equation}
    
    \begin{equation}
    \int \frac{1}{\sqrt{a^2 - x^2}}\ dx = \sin^{-1}\frac{x}{a} 
    \end{equation}

    \begin{equation}\label{eq:Winokur2}
    \int\frac{dx}{(a^2+x^2)^{3/2}}=\frac{x}{a^2\sqrt{a^2+x^2}}
    \end{equation}
        
    \begin{equation}
    \int \tan ax\ dx = -\frac{1}{a} \ln \cos ax 
    \end{equation}
    
    \begin{equation}
    \int \sec x \ dx = \ln | \sec x + \tan x | = 2 \tanh^{-1} \left (\tan \frac{x}{2} \right) 
    \end{equation}
    
\begin{equation}\label{eq:ritzert}
    \int e^{bx} \sin ax\ dx = \frac{1}{a^2+b^2}e^{bx} (b\sin ax - a\cos ax) 
    \end{equation}


\begin{equation}
    \int e^{bx} \cos ax\ dx = \frac{1}{a^2 + b^2} e^{bx} ( a \sin ax + b \cos ax ) 
    \end{equation}